Simplify definition of atoms

theories/CeresS.v
@@ -6,80 +6,62 @@ From Coq Require Import
 (* end hide *)
 
 (** S-expressions, parameterized by the type of atoms. *)
-Inductive sexp (A : Type) :=
-| Atom (a : A)
-| List (xs : list (sexp A))
+Inductive sexp_ (A : Type) :=
+| Atom_ (a : A)
+| List (xs : list (sexp_ A))
 .
 
-Arguments Atom {A} a.
+Arguments Atom_ {A} a.
 Arguments List {A} xs.
 
 (* Declare Scope sexp_scope. *)
 Delimit Scope sexp_scope with sexp.
-Bind Scope sexp_scope with sexp.
+Bind Scope sexp_scope with sexp_.
 
 Notation "[ ]" := (List nil) : sexp_scope.
-Notation "[ x ]" := (List (@cons (sexp _) x nil)) : sexp_scope.
+Notation "[ x ]" := (List (@cons (sexp_ _) x nil)) : sexp_scope.
 Notation "[ x ; y ; .. ; z ]"
-  := (List (@cons (sexp _) x (@cons (sexp _) y .. (@cons (sexp _) z nil) .. )))
+  := (List (@cons (sexp_ _) x (@cons (sexp_ _) y .. (@cons (sexp_ _) z nil) .. )))
   : sexp_scope.
 
 (** Apply a function to every atom. *)
-Fixpoint map_sexp {A B : Type} (f : A -> B) (x : sexp A) : sexp B :=
+Fixpoint map_sexp_ {A B : Type} (f : A -> B) (x : sexp_ A) : sexp_ B :=
   match x with
-  | Atom a => Atom (f a)
-  | List xs => List (map (map_sexp f) xs)
+  | Atom_ a => Atom_ (f a)
+  | List xs => List (map (map_sexp_ f) xs)
   end.
 
 (** Replace every atom with an S-expression. *)
-Fixpoint subst_sexp {A B : Type} (f : A -> sexp B) (x : sexp A) : sexp B :=
+Fixpoint subst_sexp_ {A B : Type} (f : A -> sexp_ B) (x : sexp_ A) : sexp_ B :=
   match x with
-  | Atom a => f a
-  | List xs => List (map (subst_sexp f) xs)
+  | Atom_ a => f a
+  | List xs => List (map (subst_sexp_ f) xs)
   end.
 
 (** Construct an S-expression from a list of atoms. *)
-Fixpoint sexp_of_atoms {A} (xs : list A) : sexp A :=
-  List (map Atom xs).
+Fixpoint sexp_of_atoms {A} (xs : list A) : sexp_ A :=
+  List (map Atom_ xs).
 
 (** * Default atoms *)
 
-(** Internal representation of [atom]. *)
-Variant _atom : Set :=
-| _Num (n : Z)
-| _Str (s : string)
-| _Raw (s : string)  (* Should fit in this alphabet: [A-Za-z0-9-_.'] *)
+(** Default type of atoms. [sexp_ atom] thus provides a uniform format to
+    store and exchange semi-structured data. *)
+Variant atom : Set :=
+| Num (n : Z)       (* Integers. *)
+| Str (s : string)  (* Literal strings. *)
+| Raw (s : string)  (* Simple atoms (e.g., ADT tags). *)
+                    (* Should fit in this alphabet: [A-Za-z0-9-_.']. *)
 .
 
-(** Default type of atoms. [sexp atom] thus provides a uniform format to
-    store and exchange semi-structured data.
-
-    This is an abstract type. It may be extended in the future with more
-    constructors, so pattern-matching should not be used.
-  *)
-Definition atom : Set := _atom.
-
-(** ** Constructors *)
-
-(** - [Num : Z -> atom]. Integer atoms. *)
-(** - [Str : string -> atom]. Strings (human-readable messages). *)
-(** - [Raw : string -> atom]. Raw atoms (e.g., ADT tags) *)
-
-Definition Num : Z -> atom := _Num.
-Definition Str : string -> atom := _Str.
-Definition Raw : string -> atom := _Raw.
+Notation sexp := (sexp_ atom).
+Notation Atom := (@Atom_ atom).  (* This notation helps make coercions work. *)
 
 (** Potential future extensions: binary strings, floating-point *)
 
 (** *** Coercions and notations *)
 
-Definition Atom_default : atom -> sexp atom := Atom.
-Coercion Atom_default : atom >-> sexp.
 Coercion Num : Z >-> atom.
-
-Notation ANum x := (Atom (_Num x)).
-Notation AStr x := (Atom (_Str x)).
-Notation ARaw x := (Atom (_Raw x)).
+Coercion Raw : string >-> atom.
 
 (** ** Destructors *)
 
@@ -88,25 +70,27 @@ Notation ARaw x := (Atom (_Raw x)).
 
 Definition get_Num (a : atom) : option Z :=
   match a with
-  | _Num n => Some n
+  | Num n => Some n
   | _ => None
   end.
 
 Definition get_Str (a : atom) : option string :=
   match a with
-  | _Str s => Some s
+  | Str s => Some s
   | _ => None
   end.
 
 Definition get_Raw (a : atom) : option string :=
   match a with
-  | _Raw s => Some s
+  | Raw s => Some s
   | _ => None
   end.
 
 (** ** Example *)
 Section Example.
 Import ListNotations.
+
+Local Open Scope string.
 
 (** This S-expression:
 
@@ -116,24 +100,23 @@ Import ListNotations.
   (code 418))
 >>
 
-corresponds to this [sexp atom] in Gallina:
+corresponds to this [sexp] in Gallina:
 *)
 
-Let example_1 : sexp atom :=
-  List [ Atom (Raw "example")
-       ; List [ Atom (Raw "message") ; Atom (Str "I'm a teapot") ]
-       ; List [ Atom (Raw "code") ; Atom (Num 418%Z) ]
+Let example_1 : sexp :=
+  List [ Atom "example"
+       ; List [ Atom "message" ; Atom (Str "I'm a teapot") ]
+       ; List [ Atom "code" ; Atom 418%Z ]
        ].
 
 Local Open Scope sexp.
 
-(** Or, with [Atom] and [Num] as implicit coercions and overloading the list
-    notation... *)
+(** Or, overloading the list notation... *)
 
-Let example_2 : sexp atom :=
-  [ Raw "example"
-  ; [ Raw "message" ; Str "I'm a teapot" ]
-  ; [ Raw "code" ; Num 418%Z ]
+Let example_2 : sexp :=
+  [ Atom "example"
+  ; [ Atom "message" ; Atom (Str "I'm a teapot") ]
+  ; [ Atom "code" ; Atom 418%Z ]
   ].
 
 End Example.
