theories/CeresFormat.v
@@ -10,10 +10,10 @@ From Ceres Require Import
 
 (** Helper for [string_of_sexp]. *)
 Local Definition dstring_of_sexp {A} (dstring_A : A -> DString.t)
-  : sexp A -> DString.t
-  := fix _to_dstring (x : sexp A) : DString.t :=
+  : sexp_ A -> DString.t
+  := fix _to_dstring (x : sexp_ A) : DString.t :=
     match x with
-    | Atom a => dstring_A a
+    | Atom_ a => dstring_A a
     | List nil => "()"%string
     | List (x :: xs) => fun s0 =>
         (  "("
@@ -24,17 +24,17 @@ Local Definition dstring_of_sexp {A} (dstring_A : A -> DString.t)
     end%dstring.
 
 (** Convert a [sexp] to a [string]. *)
-Definition string_of_sexp {A} (string_A : A -> string) (x : sexp A) : string :=
+Definition string_of_sexp {A} (string_A : A -> string) (x : sexp_ A) : string :=
   dstring_of_sexp string_A x ""%string.
 
 (** Convert an [atom] to a [string]. *)
 Definition string_of_atom (a : atom) : string :=
   match a with
-  | _Num n => string_of_Z n
-  | _Str s => escape_string s
-  | _Raw s => s
+  | Num n => string_of_Z n
+  | Str s => escape_string s
+  | Raw s => s
   end.
 
-(** Convert a [sexp atom] to a [string]. *)
-Definition string_of_sexpa : sexp atom -> string :=
+(** Convert a [sexp] to a [string]. *)
+Definition string_of_sexpa : sexp -> string :=
   string_of_sexp string_of_atom.
